## **Direkter Beweis** 

## **Beweis durch Wiederspruch**

## **Kontraposition**

## **VollstÃ¤ndige Induktion**

### **1. Induktionsanfang (IA)**

$$
\text{Zeige, dass die Aussage fuer n = 1}
$$



### **2. Induktionsvorausetzung (IV)**

$$
 n \in \mathbb, A(n) \Rightarrow A(n + 1)
$$

### **3. Induktionsbehauptung (IB)**

$$
A(n)
$$

### **4. Induktionsschritt (IS)**
$$
A(n+1)
$$
$$
n^{2} - 2n -1 > 0
$$
$$
n = 3
$$
$$
3^{2} -2 \cdot 3 -1 = 9 - 6 -1 = 2 > 0
$$
$$
IA: n^{2} -2n - 1 > 0\qquad n\ge 3
$$
$$
IB: (n + 1)^{2} - 2(n+1) - 1 > 0
$$
Aufgabe 2.4





































